concur/Asmselfsim.v
@@ -34,6 +34,7 @@ Lemma ros_address_lessdef:
 Proof.
   intros. unfold ros_address, Genv.find_funct. destruct ros; auto.
 Qed.
+ *)
 
 Lemma find_funct_lessdef: forall vf vf' fd,
     Genv.find_funct ge vf = Some fd ->
@@ -42,7 +43,7 @@ Lemma find_funct_lessdef: forall vf vf' fd,
 Proof.
   intros. unfold Genv.find_funct in *. inv H0; simpl in *; try congruence.
 Qed.
-
+(*
 Lemma regs_lessdef_init_regs:
   forall params vl vl',
   Val.lessdef_list vl vl' ->
@@ -103,6 +104,85 @@ Proof.
   inv H1; congruence.
 Qed.
 
+Lemma regset_lessdef_set_pair : forall rs1 rs2 p v1 v2,
+    regset_lessdef rs1 rs2 ->
+    Val.lessdef v1 v2 ->
+    regset_lessdef (set_pair p v1 rs1) (set_pair p v2 rs2).
+Proof.
+  intros. unfold set_pair. destruct p.
+  eapply regset_lessdef_set; eauto.
+  eapply regset_lessdef_set; eauto.  eapply regset_lessdef_set; eauto.
+  inv H0; constructor; eauto.
+  inv H0; constructor; eauto.
+Qed.
+
+Lemma regset_lessdef_undef_caller_save_regs : forall rs1 rs2,
+    regset_lessdef rs1 rs2 ->
+    regset_lessdef (undef_caller_save_regs rs1) (undef_caller_save_regs rs2).
+Proof.
+  intros. unfold undef_caller_save_regs. red. intros. destr; eauto.
+Qed.
+
+Lemma regset_lessdef_set_res : forall res rs1 rs2 v1 v2,
+    regset_lessdef rs1 rs2 ->
+    Val.lessdef v1 v2 ->
+    regset_lessdef (set_res res v1 rs1) (set_res res v2 rs2).
+Proof.
+  induction res; intros; simpl; eauto.
+  - eapply regset_lessdef_set; eauto.
+  - eapply IHres2. eapply IHres1. eauto.
+    inv H0; constructor.
+    inv H0; constructor.
+Qed.
+
+Ltac rs_lessdef :=
+  match goal with
+  | [ |- regset_lessdef (nextinstr_nf _ ) (nextinstr_nf _) ] =>
+      eapply regset_lessdef_nextinstr_nf; eauto
+  | [ |- regset_lessdef (nextinstr _) (nextinstr _) ] =>
+      eapply regset_lessdef_nextinstr; eauto
+  | [ |- regset_lessdef (undef_regs _ _) (undef_regs _ _) ] =>
+      eapply regset_lessdef_undef_regs; eauto
+  | [ |- regset_lessdef (undef_caller_save_regs _) (undef_caller_save_regs _) ] =>
+      eapply regset_lessdef_undef_caller_save_regs; eauto
+  | [ |- regset_lessdef (_ # _ <- _ ) (_ # _ <- _) ] =>
+      eapply regset_lessdef_set; eauto
+  | [ |- regset_lessdef (set_pair _ _ _ ) (set_pair _ _ _) ] =>
+      eapply regset_lessdef_set_pair; eauto
+  | [ |- regset_lessdef (set_res _ _ _ ) (set_res _ _ _) ] =>
+      eapply regset_lessdef_set_res; eauto
+  end.
+
+Ltac rs_lessdefs := repeat rs_lessdef.
+
+
+(** For exec_load *)
+
+Lemma eval_addrmode_lessdef : forall rs1 rs2 a se,
+    regset_lessdef rs1 rs2 ->
+    Val.lessdef (eval_addrmode se a rs1) (eval_addrmode se a rs2).
+Proof.
+Admitted.
+
+
+(** For exec_store *)
+
+
+
+
+
+
+
+(** For external calls *)
+Lemma extcall_arguments_ext: forall rs1 m1 ef args1 rs2 m2,
+    extcall_arguments rs1 m1 (ef_sig ef) args1 ->
+    Mem.extends m1 m2 ->
+    regset_lessdef rs1 rs2 ->
+    exists args2,
+      extcall_arguments rs2 m2 (ef_sig ef) args2 /\
+      Val.lessdef_list args1 args2.
+Admitted.
+
 Lemma step_correct :
   forall s1 t s2, step init_sup ge s1 t s2 ->
   forall wp s1' (MS : match_states wp s1 s1'),
@@ -110,136 +190,157 @@ Lemma step_correct :
 Proof.
   induction 1; intros; inv MS.
   - (* internal steps *)
-    Ltac 
-    Ltac solve_exec_instr := split;
-                             [econstructor; eauto using regset_lessdef_ptr; try econstructor; eauto | econstructor; eauto ].
-    destruct i; inv EXEC; eexists; solve_exec_instr.
-    + eapply regset_lessdef_nextinstr. eapply regset_lessdef_set; eauto.
-    + eapply regset_lessdef_nextinstr_nf. eapply regset_lessdef_set; eauto.
-    + eapply regset_lessdef_nextinstr_nf. eapply regset_lessdef_set; eauto.
-    + eapply regset_lessdef_nextinstr_nf. eapply regset_lessdef_set; eauto.
-    + simpl. admit. (*load*)
-    + admit.
-      eapply regset_lessdef_nextinstr_nf. eapply regset_lessdef_set; eauto.
-      
+    Ltac solve_exec_instr :=
+      eexists; split;
+      [econstructor; eauto using regset_lessdef_ptr;
+       try econstructor; eauto |
+        econstructor; eauto; try rs_lessdefs ].
     admit.
+    (*
+    destruct i; inv EXEC.   (* eexists. solve_exec_instr. *)
+    + solve_exec_instr.
+    + solve_exec_instr.
+    + solve_exec_instr.
+    + solve_exec_instr.
+    + (*exec_load*)
+      unfold exec_load in *. destr_in H1. inv H1.
+      exploit eval_addrmode_lessdef. eauto. intro.
+      exploit Mem.loadv_extends; eauto. intros [v' [Hl Hv]].
+      solve_exec_instr. simpl. unfold exec_load. rewrite Hl. reflexivity.
+      rs_lessdefs.
+    + (*exec_load*)
+      unfold exec_load in *. destr_in H1. inv H1.
+      exploit eval_addrmode_lessdef. eauto. intro.
+      exploit Mem.loadv_extends; eauto. intros [v' [Hl Hv]].
+      solve_exec_instr. simpl. unfold exec_load. rewrite Hl. reflexivity.
+      rs_lessdefs.
+    + (*exec_store*)
+      admit.
+    + admit.
+    + solve_exec_instr.
+    + solve_exec_instr.
+    + (*exec_load*)
+      unfold exec_load in *. destr_in H1. inv H1.
+      exploit eval_addrmode_lessdef. eauto. intro.
+      exploit Mem.loadv_extends; eauto. intros [v' [Hl Hv]].
+      solve_exec_instr. simpl. unfold exec_load. rewrite Hl. reflexivity.
+      rs_lessdefs.
+    + admit.
+    + solve_exec_instr.
+    + admit.
+    + admit.
+    + admit.
+    + admit.
+    + admit.
+    + admit.
+    + admit.
+    + admit.
+    + solve_exec_instr. admit.
+    + admit.
+    + solve_exec_instr. admit.
+    + admit.
+    + solve_exec_instr. admit.
+    + admit.
+    + solve_exec_instr. admit.
+    + admit.
+    + solve_exec_instr.
+      generalize (RLD rs0). intro. inv H0; constructor.
+    + solve_exec_instr. admit.
+    + solve_exec_instr. 
+     *)
   - (* builtin steps *)
-  - eexists; split; econstructor; eauto.
-  - edestruct eval_operation_lessdef as [v' [OP LD]]. 3: eauto.
-    apply regs_lessdef_regs. eauto. eauto. eexists. split.
-    eapply exec_Iop; eauto.
-    econstructor; eauto.
-    eapply set_reg_lessdef; eauto.
-  - edestruct eval_addressing_lessdef as [a' [OP LDa]]. 2: eauto.
-    apply regs_lessdef_regs. eauto.
-    edestruct Mem.loadv_extends as [v' [LD LDv]]; eauto.
-    eexists. split.
-    eapply exec_Iload; eauto.
-    econstructor; eauto.
-    eapply set_reg_lessdef; eauto.
-  - edestruct eval_addressing_lessdef as [a' [OP LDa]]. 2: eauto.
-    apply regs_lessdef_regs. eauto.
-    edestruct Mem.storev_extends as [v' [ST Hm']]; eauto.
-    exploit ext_acci_storev. apply H1. apply ST. eauto. 
-    eexists. split.
-    eapply exec_Istore; eauto.
-    econstructor; eauto. instantiate (1:= Hm'). etransitivity; eauto.
-    etransitivity; eauto.
-  - exploit ros_address_lessdef. eauto. instantiate (1:= ros). fold vf.
-    intro.
-    eexists.
-    split. eapply exec_Icall; eauto. eapply find_funct_lessdef; eauto.
-    econstructor; eauto. constructor; eauto. eapply regs_lessdef_regs. eauto.
-  - exploit ros_address_lessdef. eauto. instantiate (1:= ros). fold vf.
-    intro. exploit Mem.free_parallel_extends; eauto.
-    intros [tm' [FREE Hm']]. exploit ext_acci_free. apply H2. apply FREE.  intro AI.
-    eexists.
-    split. eapply exec_Itailcall; eauto. eapply find_funct_lessdef; eauto.
-    econstructor; eauto. eapply regs_lessdef_regs. eauto. instantiate (1:= Hm').
-    etransitivity; eauto. etransitivity; eauto.
-  - edestruct eval_builtin_args_lessdef as [vargs' [EV ARGSLD]]. apply RLD. eauto. eauto.
-    exploit external_call_mem_extends; eauto. intros (vres' & m'1 & A & B & C & D & E).
-    assert (ACCI: ext_acci (extw m m'0 Hm) (extw m' m'1 C)).
+    exploit (eval_builtin_args_rel ext (extw m m'0 Hm)); simpl.
+    instantiate (1:= se). eapply Genv.match_stbls_id.
+    red. intros. 
+    eapply val_inject_id. apply RLD. eapply val_inject_id.
+    generalize (RLD RSP). eauto. constructor. eauto.
+    intros [vargs' [EVAL' ARGSL]].
+    exploit external_call_mem_extends; eauto.
+    apply val_inject_list_lessdef; eauto.
+    intros (res' & m'1 & CALL' & A & B & C & D).
+    assert (ACCI: ext_acci (extw m m'0 Hm) (extw m' m'1 B)).
     econstructor; eauto using external_call_tid, external_call_support.
     red. intros. eauto using external_call_max_perm.
     red. intros. eauto using external_call_max_perm.
-    eexists. split. eapply exec_Ibuiltin; eauto. econstructor; eauto.
-    apply set_res_lessdef; eauto. instantiate (1:= C).
+    eexists. split. eapply exec_step_builtin; eauto using regset_lessdef_ptr.
+    econstructor; eauto. rs_lessdefs.
     etransitivity; eauto. etransitivity; eauto.
-  - exploit eval_condition_lessdef. apply regs_lessdef_regs. eauto. eauto. eauto.
-    intro. eexists. split. eapply exec_Icond; eauto. econstructor; eauto.
-  - specialize (RLD arg) as ARGLD. rewrite H0 in ARGLD. inv ARGLD.
-    eexists. split.
-    eapply exec_Ijumptable; eauto. econstructor; eauto.
-  - exploit Mem.free_parallel_extends; eauto. intros [m'1 [FREE Hm1]].
-    exploit ext_acci_free. apply H0. apply FREE. intro.
-    eexists. split. eapply exec_Ireturn; eauto. econstructor; eauto.
-    destruct or;  eauto. instantiate (1:= Hm1). etransitivity; eauto. etransitivity; eauto.
-  - exploit Mem.alloc_extends; eauto. reflexivity. reflexivity.
-    intros [m'1 [ALLOC Hm1]]. exploit ext_acci_alloc. apply H. eauto. intro.
-    eexists. split. eapply exec_function_internal; eauto. eapply find_funct_lessdef; eauto.
-    econstructor; eauto. apply regs_lessdef_init_regs. eauto. instantiate (1:= Hm1).
-    etransitivity; eauto. etransitivity; eauto.
-  - exploit external_call_mem_extends; eauto. intros (vres' & m'1 & A & B & C & D & E).
-    assert (ACCI: ext_acci (extw m m'0 Hm) (extw m' m'1 C)).
+  - exploit extcall_arguments_ext; eauto.
+    intros [args' [ARGS' Hll]].
+    exploit external_call_mem_extends; eauto.
+    intros (res' & m'1 & CALL' & A & B & C & D).
+    assert (ACCI: ext_acci (extw m m'0 Hm) (extw m' m'1 B)).
     econstructor; eauto using external_call_tid, external_call_support.
     red. intros. eauto using external_call_max_perm.
     red. intros. eauto using external_call_max_perm.
-    eexists. split. eapply exec_function_external; eauto. eapply find_funct_lessdef; eauto.
-    econstructor; eauto. instantiate (1:= C).
+    eexists. split. eapply exec_step_external; eauto using regset_lessdef_ptr.
+    unfold inner_sp in *. destr_in ISP. exploit regset_lessdef_ptr.
+    eauto. apply Heqv. intro. rewrite H0. rewrite ISP. reflexivity.
+    econstructor; eauto. rs_lessdefs.
     etransitivity; eauto. etransitivity; eauto.
-  - inv STACKS. eexists. split. eapply exec_return; eauto. econstructor; eauto.
-    apply set_reg_lessdef; eauto.
-Qed.
+Admitted. 
       
 Lemma initial_correct:
-  forall q1 q2 st1, GS.match_query c_ext w q1 q2 -> initial_state ge q1 st1 ->
+  forall q1 q2 st1, GS.match_query asm_ext w q1 q2 -> initial_state ge q1 st1 ->
                exists st2, initial_state ge q2 st2 /\ match_states (get w) st1 st2.
 Proof.
-  intros. destruct H. inv H2. clear Hm1. inv H0. CKLR.uncklr. 
+  intros. destruct H0. destruct q2. inv H. inv H4. clear Hm1.
+  rewrite <- H in *. simpl in H3.
   eexists. split. econstructor; eauto. eapply find_funct_lessdef; eauto.
-  econstructor; eauto. constructor. instantiate (1:= Hm).
-  constructor; eauto; red; intros; eauto. rewrite <- H4. reflexivity.
+  eapply val_inject_id; eauto.
+  generalize (H3 RSP). intro. inv H4; congruence.
+  generalize (H3 RA). intro. inv H4; congruence.
+  econstructor; eauto. red. intros. eapply val_inject_id; eauto.
+  instantiate (1:= Hm).
+  constructor; eauto; red; intros; eauto. rewrite <- H. reflexivity.
 Qed.
 
 Lemma final_correct:
   forall wp st1 st2 r1, match_states wp st1 st2 -> final_state st1 r1 ->
                    exists r2 wp', final_state st2 r2 /\ (get w) o-> wp' /\ ext_acci wp wp' /\
-                                                               GS.match_reply (c_ext) (CallconvBig.set w wp') r1 r2.
+                                                               GS.match_reply (asm_ext) (CallconvBig.set w wp') r1 r2.
 Proof.
-  intros. inv H0. inv H. inv STACKS.
+  intros. inv H0. inv H.
   eexists. exists (extw m m' Hm). split.
   - constructor.
-  - split. auto. split. auto. constructor; CKLR.uncklr; cbn; auto. constructor.
+  - split. auto. split. auto. constructor; cbn; auto.
+    intros. eapply val_inject_id; eauto.
+    constructor.
 Qed.
 
 Lemma external_correct:
   forall wp st1 st2 q1, match_states wp st1 st2 -> at_external ge st1 q1 ->
-  exists wx q2, at_external ge st2 q2 /\ ext_acci wp (get wx) /\  GS.match_query (c_ext) wx q1 q2 /\ se = se /\
-  forall r1 r2 st1' wp'', (get wx) o-> wp'' -> GS.match_reply (c_ext) (CallconvBig.set w wp'') r1 r2 -> after_external st1 r1 st1' ->
-  exists st2', after_external st2 r2 st2' /\ match_states wp'' st1' st2'.
+  exists wx q2, at_external ge st2 q2 /\ ext_acci wp (get wx) /\  GS.match_query (asm_ext) wx q1 q2 /\ se = se /\
+  forall r1 r2 st1' wp'', (get wx) o-> wp'' -> GS.match_reply (asm_ext) (CallconvBig.set w wp'') r1 r2 -> after_external init_sup st1 r1 st1' ->
+  exists st2', after_external init_sup st2 r2 st2' /\ match_states wp'' st1' st2'.
 Proof.
   intros wp st1 st2 q1 Hst Hq1. destruct Hq1. inv Hst.
   exists (extw m m' Hm). eexists. intuition idtac.
   - econstructor; eauto. eapply find_funct_lessdef; eauto.
-  - constructor; CKLR.uncklr; auto. constructor.
-    destruct vf; cbn in *; congruence.
-  - inv H1. inv H2. inv H4. CKLR.uncklr.
-    exists (Returnstate s' vres2 m2'). split. econstructor; eauto. simpl in H1. inv H1.
-    econstructor; eauto. reflexivity. etransitivity. eauto. simpl in H0. eauto.
+  - constructor; CKLR.uncklr; auto. simpl. intros.
+    eapply val_inject_id; eauto.
+    constructor.
+  - inv H2. destruct r2. inv H1. simpl in H2. simpl in H0, H3. inv H3.
+    eexists. split. econstructor; eauto. inv H0. eauto.
+    unfold inner_sp in *. generalize (H2 RSP). intro. apply val_inject_id in H1.
+    destr_in H8. inv H1. rewrite H8. reflexivity.
+    econstructor; eauto. red. intros. apply val_inject_id; eauto.
+    reflexivity. etransitivity. eauto. simpl in H0. inv H0. constructor; eauto.
 Qed.
 
 End EXT.
 
 Theorem RTL_ext_selfsim prog :
-  GS.forward_simulation (c_ext) (RTL.semantics prog) (RTL.semantics prog).
+  GS.forward_simulation (asm_ext) (Asm.semantics prog) (Asm.semantics prog).
 Proof.
   constructor.
   eapply GS.Forward_simulation.
   + reflexivity.
   + intros se1 se2 w Hse Hse1. cbn -[semantics] in *.
   eapply GS.forward_simulation_step; subst.
-  - destruct 1. CKLR.uncklr. destruct H; cbn; try congruence.
+  - intros. CKLR.uncklr. destruct q1, q2. inv H. simpl.
+    simpl in H0. generalize (H0 PC). intro.
+    apply val_inject_id in H. inv H. reflexivity. 
   - eapply initial_correct; eauto.
   - eapply final_correct; eauto.
   - eapply external_correct; eauto.
